\include{headerueb}
\include{header}
\include{info}


\newcommand{\nr}{8}

\begin{document}
\section*{Aufgabe 1}

\begin{eqnarray}
(\lambda x . y) z& \overset\beta\to & y\\
\downarrow^{\alpha'}&&\\
(\lambda y . y) z& \overset\beta\to & z
\end{eqnarray}

\section*{Aufgabe 2}
\begin{eqnarray}
(\lambda x . \lambda y . x) y  & \overset{\alpha,\beta}\to & \lambda z . y\\
\downarrow^{\beta'}&\\
\lambda y . y &&
\end{eqnarray}

\section*{Aufgabe 3}
\begin{equation}
(\lambda x . x x x)(\lambda x . x x x)
\end{equation}

\section*{Aufgabe 4}
\begin{enumerate}[a)]
\item \begin{equation}
\lambda F x . F;F;F x : [D \to D] \to D \to D
\end{equation}

\item \begin{equation}
\lambda L g . \langle g; \pi_1 L, g; \pi_2 L, g; \pi_3 L, g; \pi_4 L \rangle : D^* \to [D \to D] \to D^*
\end{equation}

\item \begin{equation}
\lambda f . \lambda \langle x,y \rangle . f x y : [D \to D \to D] \to [(D \times D) \to D]
\end{equation}

\end{enumerate}

\end{document}
